TaplLean/STLC/Internal.lean
@@ -22,12 +22,12 @@ notation:90 "λ" x " : " T " , " t => Term.abs x T t
 inductive WellTyped : TyEnv → Term → Ty → Prop where
   | wt_tru : ∀ Γ, WellTyped Γ Term.tru Ty.TBool
   | wt_fls : ∀ Γ, WellTyped Γ Term.fls Ty.TBool
-  | wt_ite : ∀ Γ t1 t2 t3 T,
+  | wt_ite : ∀ {Γ t1 t2 t3 T},
       WellTyped Γ t1 Ty.TBool →
       WellTyped Γ t2 T →
       WellTyped Γ t3 T →
       WellTyped Γ (Term.ite t1 t2 t3) T
-  | wt_var : ∀ Γ x T, Γ x = some T → WellTyped Γ (Term.var x) T
+  | wt_var : ∀ {Γ x T}, Γ x = some T → WellTyped Γ (Term.var x) T
   | wt_abs : ∀ Γ x t1 T1 T2,
       WellTyped (x |→ T2; Γ) t1 T1 →
       WellTyped Γ (λ x : T2 , t1) (T2 :-> T1)
